<?xml version="1.0"?>


<!DOCTYPE rdf:RDF [
    <!ENTITY terms "http://purl.org/dc/terms/" >
    <!ENTITY owl "http://www.w3.org/2002/07/owl#" >
    <!ENTITY dc "http://purl.org/dc/elements/1.1/" >
    <!ENTITY xsd "http://www.w3.org/2001/XMLSchema#" >
    <!ENTITY rdfs "http://www.w3.org/2000/01/rdf-schema#" >
    <!ENTITY rdf "http://www.w3.org/1999/02/22-rdf-syntax-ns#" >
]>


<rdf:RDF xmlns="http://aligned-project.eu/ontologies/sdo#"
     xml:base="http://aligned-project.eu/ontologies/sdo"
     xmlns:rdf="http://www.w3.org/1999/02/22-rdf-syntax-ns#"
     xmlns:terms="http://purl.org/dc/terms/"
     xmlns:owl="http://www.w3.org/2002/07/owl#"
     xmlns:xsd="http://www.w3.org/2001/XMLSchema#"
     xmlns:rdfs="http://www.w3.org/2000/01/rdf-schema#"
     xmlns:dc="http://purl.org/dc/elements/1.1/">
    <owl:Ontology rdf:about="http://aligned-project.eu/ontologies/sdo">
        <owl:versionInfo rdf:datatype="&xsd;decimal">1.0</owl:versionInfo>
        <terms:title>Seshat Domain Ontology</terms:title>
        <dc:publisher>Trinity College Dublin</dc:publisher>
        <dc:description rdf:resource="https://www.scss.tcd.ie/~bozicb/images/sdo.png"/>
        <rdfs:comment>This ontology provides a description of the data lifecycle for Seshat.</rdfs:comment>
        <dc:date>09-07-2015</dc:date>
        <dc:contributor xml:lang="cs.tcd.ie)">Kevin C. Feeney (kevin.feeney</dc:contributor>
        <dc:contributor xml:lang="cs.tcd.ie)">Rob Brennan (rob.brennan</dc:contributor>
        <dc:description>The purpose of the Seshat Domain Ontology is to provide a set of concrete entities, agents, activities, and roles to represent the Seshat data engineering process. It is based on the general Data Lifecycle Ontology.

This ontology imports the W3C PROV ontology available at http://www.w3c.org/TR/prov-o/. It is derived from the Data Lifecycle Ontology available at http://aligned-project.eu/ontologies/dlo.</dc:description>
        <dc:creator xml:lang="scss.tcd.ie)">Bojan Božić (bozicb</dc:creator>
        <owl:imports rdf:resource="https://w3id.org/dlo"/>
        <owl:imports rdf:resource="http://www.w3.org/ns/prov-o-20130430"/>
    </owl:Ontology>
    


    <!-- 
    ///////////////////////////////////////////////////////////////////////////////////////
    //
    // Classes
    //
    ///////////////////////////////////////////////////////////////////////////////////////
     -->

    


    <!-- http://aligned-project.eu/ontologies/dlo#Process -->

    <rdf:Description rdf:about="http://aligned-project.eu/ontologies/dlo#Process">
        <rdfs:subClassOf rdf:resource="http://www.w3.org/ns/prov#Activity"/>
    </rdf:Description>
    


    <!-- http://aligned-project.eu/ontologies/sdo#Candidate -->

    <owl:Class rdf:about="http://aligned-project.eu/ontologies/sdo#Candidate">
        <rdfs:label>Candidate</rdfs:label>
        <rdfs:subClassOf rdf:resource="http://www.w3.org/ns/prov#Entity"/>
        <rdfs:comment>A dataset which is potentially going to be included into the database.</rdfs:comment>
    </owl:Class>
    


    <!-- http://aligned-project.eu/ontologies/sdo#Consumer -->

    <owl:Class rdf:about="http://aligned-project.eu/ontologies/sdo#Consumer">
        <rdfs:label>Consumer</rdfs:label>
        <rdfs:subClassOf rdf:resource="http://www.w3.org/ns/prov#Role"/>
        <rdfs:comment>A person or software agent who consumes data from the system.</rdfs:comment>
    </owl:Class>
    


    <!-- http://aligned-project.eu/ontologies/sdo#Creation -->

    <owl:Class rdf:about="http://aligned-project.eu/ontologies/sdo#Creation">
        <rdfs:label>Creation</rdfs:label>
        <rdfs:subClassOf rdf:resource="http://aligned-project.eu/ontologies/dlo#Process"/>
        <rdfs:comment>Input of new data through a human (e.g. user/domain expert) or machine (e.g. sensor) source.</rdfs:comment>
    </owl:Class>
    


    <!-- http://aligned-project.eu/ontologies/sdo#DataCollection -->

    <owl:Class rdf:about="http://aligned-project.eu/ontologies/sdo#DataCollection">
        <rdfs:label>Data Collection</rdfs:label>
        <rdfs:subClassOf rdf:resource="http://aligned-project.eu/ontologies/dlo#Process"/>
        <rdfs:comment>Automatic or semi-automatic input of new data (e.g. through a harvester).</rdfs:comment>
    </owl:Class>
    


    <!-- http://aligned-project.eu/ontologies/sdo#Elaboration -->

    <owl:Class rdf:about="http://aligned-project.eu/ontologies/sdo#Elaboration">
        <rdfs:label>Elaboration</rdfs:label>
        <rdfs:subClassOf rdf:resource="http://aligned-project.eu/ontologies/dlo#Process"/>
        <rdfs:comment>Addition of new information to already existing data.</rdfs:comment>
    </owl:Class>
    


    <!-- http://aligned-project.eu/ontologies/sdo#Extraction -->

    <owl:Class rdf:about="http://aligned-project.eu/ontologies/sdo#Extraction">
        <rdfs:label>Extraction</rdfs:label>
        <rdfs:subClassOf rdf:resource="http://aligned-project.eu/ontologies/dlo#Process"/>
        <rdfs:comment>Gathering of specific information from structured data sources.</rdfs:comment>
    </owl:Class>
    


    <!-- http://aligned-project.eu/ontologies/sdo#Filtering -->

    <owl:Class rdf:about="http://aligned-project.eu/ontologies/sdo#Filtering">
        <rdfs:label>Filtering</rdfs:label>
        <rdfs:subClassOf rdf:resource="http://aligned-project.eu/ontologies/dlo#Process"/>
        <rdfs:comment>Selection of specific information out of a large data set or data base.</rdfs:comment>
    </owl:Class>
    


    <!-- http://aligned-project.eu/ontologies/sdo#HTML -->

    <owl:Class rdf:about="http://aligned-project.eu/ontologies/sdo#HTML">
        <rdfs:label>HTML</rdfs:label>
        <rdfs:subClassOf rdf:resource="http://www.w3.org/ns/prov#Entity"/>
        <rdfs:comment>An HTML resource (e.g. a Website).</rdfs:comment>
    </owl:Class>
    


    <!-- http://aligned-project.eu/ontologies/sdo#Interpretation -->

    <owl:Class rdf:about="http://aligned-project.eu/ontologies/sdo#Interpretation">
        <rdfs:label>Interpretation</rdfs:label>
        <rdfs:subClassOf rdf:resource="http://www.w3.org/ns/prov#Entity"/>
        <rdfs:comment>The way a dataset is actually saved into the system (also includes the format).</rdfs:comment>
    </owl:Class>
    


    <!-- http://aligned-project.eu/ontologies/sdo#JStore -->

    <owl:Class rdf:about="http://aligned-project.eu/ontologies/sdo#JStore">
        <rdfs:label>JStore</rdfs:label>
        <rdfs:subClassOf rdf:resource="http://www.w3.org/ns/prov#Entity"/>
        <rdfs:comment>jQuery based client-side storage management.</rdfs:comment>
    </owl:Class>
    


    <!-- http://aligned-project.eu/ontologies/sdo#Merging -->

    <owl:Class rdf:about="http://aligned-project.eu/ontologies/sdo#Merging">
        <rdfs:label>Merging</rdfs:label>
        <rdfs:subClassOf rdf:resource="http://aligned-project.eu/ontologies/dlo#Process"/>
        <rdfs:comment>Putting data from different sources and/or from spanning different but overlapping knowledge together.</rdfs:comment>
    </owl:Class>
    


    <!-- http://aligned-project.eu/ontologies/sdo#MetaReport -->

    <owl:Class rdf:about="http://aligned-project.eu/ontologies/sdo#MetaReport">
        <rdfs:label>Meta-Report</rdfs:label>
        <rdfs:subClassOf rdf:resource="http://www.w3.org/ns/prov#Entity"/>
        <rdfs:comment>Data about a certain report.</rdfs:comment>
    </owl:Class>
    


    <!-- http://aligned-project.eu/ontologies/sdo#Prefiltering -->

    <owl:Class rdf:about="http://aligned-project.eu/ontologies/sdo#Prefiltering">
        <rdfs:label>Prefiltering</rdfs:label>
        <rdfs:subClassOf rdf:resource="http://aligned-project.eu/ontologies/dlo#Process"/>
        <rdfs:comment>Preparation for filtering in the case the data set is too big to be filtered in one single step.</rdfs:comment>
    </owl:Class>
    


    <!-- http://aligned-project.eu/ontologies/sdo#Processor -->

    <owl:Class rdf:about="http://aligned-project.eu/ontologies/sdo#Processor">
        <rdfs:label>Processor</rdfs:label>
        <rdfs:subClassOf rdf:resource="http://www.w3.org/ns/prov#Role"/>
        <rdfs:comment>A person or software agent who changes data in the system.</rdfs:comment>
    </owl:Class>
    


    <!-- http://aligned-project.eu/ontologies/sdo#Producer -->

    <owl:Class rdf:about="http://aligned-project.eu/ontologies/sdo#Producer">
        <rdfs:label>Producer</rdfs:label>
        <rdfs:subClassOf rdf:resource="http://www.w3.org/ns/prov#Role"/>
        <rdfs:comment>A person or software agent who produces new data and provides them to the system.</rdfs:comment>
    </owl:Class>
    


    <!-- http://aligned-project.eu/ontologies/sdo#Publishing -->

    <owl:Class rdf:about="http://aligned-project.eu/ontologies/sdo#Publishing">
        <rdfs:label>Publishing</rdfs:label>
        <rdfs:subClassOf rdf:resource="http://aligned-project.eu/ontologies/dlo#Process"/>
        <rdfs:comment>Publishing of data on the Web in a structured format.</rdfs:comment>
    </owl:Class>
    


    <!-- http://aligned-project.eu/ontologies/sdo#Querying -->

    <owl:Class rdf:about="http://aligned-project.eu/ontologies/sdo#Querying">
        <rdfs:label>Querying</rdfs:label>
        <rdfs:subClassOf rdf:resource="http://aligned-project.eu/ontologies/dlo#Process"/>
        <rdfs:comment>Sending queries to a database and retrieving results based on the query criteria.</rdfs:comment>
    </owl:Class>
    


    <!-- http://aligned-project.eu/ontologies/sdo#Report -->

    <owl:Class rdf:about="http://aligned-project.eu/ontologies/sdo#Report">
        <rdfs:label>Report</rdfs:label>
        <rdfs:subClassOf rdf:resource="http://www.w3.org/ns/prov#Entity"/>
        <rdfs:comment>A dataset actually included into the database.</rdfs:comment>
    </owl:Class>
    


    <!-- http://aligned-project.eu/ontologies/sdo#Revision -->

    <owl:Class rdf:about="http://aligned-project.eu/ontologies/sdo#Revision">
        <rdfs:label>Revision</rdfs:label>
        <rdfs:subClassOf rdf:resource="http://aligned-project.eu/ontologies/dlo#Process"/>
        <rdfs:comment>Improvement of quality of data through a user.</rdfs:comment>
    </owl:Class>
    


    <!-- http://aligned-project.eu/ontologies/sdo#Updating -->

    <owl:Class rdf:about="http://aligned-project.eu/ontologies/sdo#Updating">
        <rdfs:label>Updating</rdfs:label>
        <rdfs:subClassOf rdf:resource="http://aligned-project.eu/ontologies/dlo#Process"/>
        <rdfs:comment>Adding new information or modifying existing data.</rdfs:comment>
    </owl:Class>
    


    <!-- http://aligned-project.eu/ontologies/sdo#WebResource -->

    <owl:Class rdf:about="http://aligned-project.eu/ontologies/sdo#WebResource">
        <rdfs:label>Web Resource</rdfs:label>
        <rdfs:subClassOf rdf:resource="http://www.w3.org/ns/prov#Entity"/>
        <rdfs:comment>A general resource that can be identified by a URL and is located on the Web.</rdfs:comment>
    </owl:Class>
    


    <!-- http://aligned-project.eu/ontologies/sdo#Wiki -->

    <owl:Class rdf:about="http://aligned-project.eu/ontologies/sdo#Wiki">
        <rdfs:label>Wiki</rdfs:label>
        <rdfs:subClassOf rdf:resource="http://www.w3.org/ns/prov#Entity"/>
        <rdfs:comment>A wiki page providing data which can be used as input.</rdfs:comment>
    </owl:Class>
</rdf:RDF>



<!-- Generated by the OWL API (version 3.5.0) http://owlapi.sourceforge.net -->

